Added utility functions to HyperGraph and TensorGraph

theories/GraphCore/HyperGraph.v
@@ -2,13 +2,11 @@ Require Export Aux_pos TESyntax.
 From stdpp Require Export list sorting fin_maps.
 From stdpp Require Export pmap gmap.
 
+
+(* A hyper edge is an indicator for the edge type and the source and target vertices *)
+Notation HyperEdge T := (T * list positive * list positive)%type.
 (* A HyperGraph representation where edges have a type T and the graph is represented as a map of positives to (edge_data, input_vertices, output_vertices) *)
 (* Notation HyperGraph T := (Pmap (T * list positive * list positive)).
-
-(* Instance Union_hypergraph {T} : Union (HyperGraph T) := {
-  union := union
-}. *)
-
 
 Definition disj_union_hypergraph {T} (hg0 hg1 : HyperGraph T) : HyperGraph T :=
   (kmap (bcons false) (relabel_abs (bcons false) <$> hg0) ∪ 
@@ -17,6 +15,34 @@ Definition disj_union_hypergraph {T} (hg0 hg1 : HyperGraph T) : HyperGraph T :=
 Instance Disjoint_union_hypergraph {T} : DisjUnion (HyperGraph T) :={
   disj_union := disj_union_hypergraph
 }.
+
+Definition targets {T} (he : HyperEdge T) : list positive :=
+  snd he.
+Definition sources {T} (he : HyperEdge T) : list positive :=
+  snd (fst he).
+
+Definition in_target {T} (v e : positive) (hg : HyperGraph T) :=
+  is_Some (In v <$> (targets <$> (hg !! e))).
+
+Lemma in_target_means_lookup_succeeds {T} (v e : positive) (hg : HyperGraph T) :
+  in_target v e hg -> is_Some (hg !! e).
+Proof.
+  intros.
+  inversion H.
+  destruct (hg !! e).
+  - easy.
+  - contradict H0; easy. 
+Qed.
+
+Definition in_source {T} (v e : positive) (hg : HyperGraph T) :=
+  is_Some (In v <$> (sources <$> (hg !! e))).
+
+Definition predecessor {T} (h h' : positive) (hg : HyperGraph T) :=
+  exists x, in_target x h hg /\ in_source x h' hg.
+
+Definition successor {T} (h h' : positive) (hg : HyperGraph T) :=
+  exists x, in_target x h' hg /\ in_source x h hg.
+
 
 Local Open Scope positive.
 Definition example_disj_union : HyperGraph positive := 
